pushing the tactic language forward results in problems
- need to add contexts

theories/LambdaWt/WtTactic.v
@@ -1,11 +1,16 @@
 Require Import Coq.Lists.List.
+Require Import ExtLib.Structures.Functor.
+Require Import ExtLib.Structures.Applicative.
+Require Import ExtLib.Structures.Monads.
 Require Import ExtLib.Data.Member.
 Require Import ExtLib.Data.HList.
 Require Import ChargeCore.Logics.ILogic.
+Require Import ChargeCore.Tactics.Tactics.
 Require Import MirrorCore.LambdaWt.MLogic.
 Require Import MirrorCore.LambdaWt.WtExpr.
 Require Import MirrorCore.LambdaWt.SubstWt.
 Require Import MirrorCore.LambdaWt.WtMigrator.
+Require Import MirrorCore.LambdaWt.Unify.
 
 Set Implicit Arguments.
 Set Strict Implicit.
@@ -19,128 +24,7 @@ Section simple_dep_types.
   Variable EsymbolD : forall t, Esymbol t -> typeD TsymbolD t.
   Variable Esymbol_eq_dec : forall t (a b : Esymbol t), {a = b} + {a <> b}.
 
-  Context (Inst : list _ -> Type)
-          {Inst_Inst : Instantiation TsymbolD Esymbol Inst}.
-
-  Variable tyProp : type Tsymbol.
-  Context {tyPropL : ILogicOps (typeD TsymbolD tyProp)}.
-  Context {tyPropLo : ILogic (typeD TsymbolD tyProp)}.
-
-  Section logicT.
-
-    Fixpoint foralls_prop (ts : list (type Tsymbol))
-    : (hlist (typeD TsymbolD) ts -> typeD TsymbolD tyProp) ->
-      typeD TsymbolD tyProp :=
-      match ts with
-      | nil => fun k => k Hnil
-      | t :: ts => fun k =>
-        foralls_prop (fun vs =>
-                        lforall (fun v => k (Hcons v vs)))
-      end.
-
-    Fixpoint foralls_uvar_prop (ts : list (Tuvar Tsymbol))
-    : (hlist (fun tst => hlist (typeD TsymbolD) (fst tst) -> typeD TsymbolD (snd tst)) ts -> Prop) ->
-      Prop :=
-      match ts with
-      | nil => fun k => k Hnil
-      | t :: ts => fun k =>
-        foralls_uvar_prop (fun vs => forall v, k (Hcons v vs))
-      end.
-
-    Require Import ExtLib.Structures.Applicative.
-
-    Section impls.
-      Context {tus : list (Tuvar Tsymbol)} {tvs : list (type Tsymbol)}.
-      Fixpoint impls_prop (ts : list (typeD TsymbolD tyProp))
-               (post : typeD TsymbolD tyProp)
-      : typeD TsymbolD tyProp :=
-        match ts with
-        | nil => post
-        | t :: ts =>
-          limpl t (impls_prop ts post)
-        end.
-    End impls.
-
-    Variable m : Type -> Type.
-
-    Inductive wtgoal tus tvs : Type :=
-    | wtSolved : wtgoal tus tvs
-    | wtGoal   : wtexpr Esymbol tus tvs tyProp -> wtgoal tus tvs
-    | wtConj   : wtgoal tus tvs -> wtgoal tus tvs -> wtgoal tus tvs
-    | wtHyp    : wtexpr Esymbol tus tvs tyProp -> wtgoal tus tvs -> wtgoal tus tvs
-    | wtAll    : forall t, wtgoal tus (t :: tvs) -> wtgoal tus tvs.
-
-    Fixpoint wtgoalD {tus tvs} (g : wtgoal tus tvs) {struct g}
-    : exprT TsymbolD tus tvs (typeD TsymbolD tyProp) :=
-      match g with
-      | wtSolved _ _ => pure ltrue
-      | wtGoal g => wtexprD EsymbolD g
-      | wtConj l r =>
-        ap (ap (pure land) (wtgoalD l)) (wtgoalD r)
-      | wtHyp h g => ap (ap (pure limpl) (wtexprD EsymbolD h)) (wtgoalD g)
-      | @wtAll _ _ t g =>
-        let gD := wtgoalD g in
-        ap (T:=exprT TsymbolD tus tvs) (pure (@lforall _ _ (typeD TsymbolD t)))
-           (fun us vs v => gD us (Hcons v vs))
-      end.
-
-    Variables Pre Post : list (Tuvar Tsymbol) -> list (type Tsymbol) -> Type.
-
-    Record resultC tus tvs : Type := mkResultC
-    { resultUs       : _
-    ; result         : Post resultUs tvs
-    ; resultPrems    : list (wtexpr Esymbol resultUs tvs tyProp)
-    ; resultSubst    : Inst resultUs
-    ; resultMigrator : migrator Esymbol tus resultUs }.
-    Arguments mkResultC {_ _} _ _ _ _ _ : clear implicits.
-
-    Definition logicC tus tvs : Type :=
-      forall
-        (prems : list (wtexpr Esymbol tus tvs tyProp))
-        (inst  : Inst tus)
-        (goal  : Pre tus tvs),
-        m (resultC tus tvs).
-
-    (** NOTE: [logicT] does not form a monad due to the generalization
-     **       over the indices.
-     **)
-    Definition logicT : Type :=
-      forall tus tvs, logicC tus tvs.
-
-    Variable PreD
-    : forall {tus tvs}, Pre tus tvs ->
-                        exprT TsymbolD tus tvs (typeD TsymbolD tyProp).
-    Variable PostD
-    : forall {tus tvs}, Post tus tvs ->
-                        exprT TsymbolD tus tvs (typeD TsymbolD tyProp).
-    Variable mD : forall T (TD : T -> Prop), m T -> Prop.
-
-    Definition logicC_spec {tus tvs} (c : logicC tus tvs) : Prop :=
-      forall prems goal inst result,
-        c prems inst goal = result ->
-        mD (fun t =>
-              match t with
-              | mkResultC tus' post prems' inst' trans =>
-                Inst_evolves trans inst inst' /\
-                @foralls_uvar_prop tus' (fun us' =>
-                  let us := migrate_env EsymbolD trans us' in
-                  InstD inst' us' ->
-                  lentails ltrue
-                    (@foralls_prop tvs (fun vs =>
-                       limpl (impls_prop
-                                (map (fun p => wtexprD EsymbolD p us' vs) prems')
-                                (@PostD _ _ post us' vs))
-                             (impls_prop
-                                (map (fun p => wtexprD EsymbolD p us vs) prems)
-                                (@PreD  _ _ goal us  vs)))))
-              end)
-           result.
-
-    Definition logicT_spec (l : logicT) : Prop :=
-      forall tus tvs,
-        logicC_spec (l tus tvs).
-  End logicT.
-
+  (** TODO(gmalecha): Move **)
   Definition exprR tus tvs (T : Type) (R : T -> T -> Prop)
   : exprT TsymbolD tus tvs T -> exprT TsymbolD tus tvs T -> Prop :=
     fun v1 v2 =>
@@ -164,6 +48,198 @@ Section simple_dep_types.
     unfold wtRespectful, Ap_exprT, exprR.
     intros; eauto.
   Defined.
+
+
+  Context (Inst : list _ -> Type)
+          {Inst_Inst : Instantiation TsymbolD Esymbol Inst}.
+
+  Variable tyProp : type Tsymbol.
+  Context {tyPropL : ILogicOps (typeD TsymbolD tyProp)}.
+  Context {tyPropLo : ILogic (typeD TsymbolD tyProp)}.
+
+  Section logicM.
+
+    Fixpoint foralls_prop (ts : list (type Tsymbol))
+    : (hlist (typeD TsymbolD) ts -> typeD TsymbolD tyProp) ->
+      typeD TsymbolD tyProp :=
+      match ts with
+      | nil => fun k => k Hnil
+      | t :: ts => fun k =>
+        foralls_prop (fun vs =>
+                        lforall (fun v => k (Hcons v vs)))
+      end.
+
+    Fixpoint foralls_uvar_prop (ts : list (Tuvar Tsymbol))
+    : (hlist (fun tst => hlist (typeD TsymbolD) (fst tst) -> typeD TsymbolD (snd tst)) ts -> Prop) ->
+      Prop :=
+      match ts with
+      | nil => fun k => k Hnil
+      | t :: ts => fun k =>
+        foralls_uvar_prop (fun vs => forall v, k (Hcons v vs))
+      end.
+
+    Section impls.
+      Context {tus : list (Tuvar Tsymbol)} {tvs : list (type Tsymbol)}.
+      Fixpoint impls_prop (ts : list (typeD TsymbolD tyProp))
+               (post : typeD TsymbolD tyProp)
+      : typeD TsymbolD tyProp :=
+        match ts with
+        | nil => post
+        | t :: ts =>
+          limpl t (impls_prop ts post)
+        end.
+    End impls.
+
+    Variable m : Type -> Type.
+
+    Inductive wtgoal tus tvs : Type :=
+    | wtSolved : wtgoal tus tvs
+    | wtGoal   : wtexpr Esymbol tus tvs tyProp -> wtgoal tus tvs
+    | wtConj   : wtgoal tus tvs -> wtgoal tus tvs -> wtgoal tus tvs
+    | wtHyp    : wtexpr Esymbol tus tvs tyProp -> wtgoal tus tvs -> wtgoal tus tvs
+    | wtAll    : forall t, wtgoal tus (t :: tvs) -> wtgoal tus tvs.
+    Arguments wtSolved {_ _}.
+    Arguments wtGoal {_ _} _.
+    Arguments wtConj {_ _} _ _.
+    Arguments wtHyp {_ _} _ _.
+    Arguments wtAll {_ _} _ _.
+
+    Section wtgoal_subst.
+      Context {tus tus' : list (Tuvar Tsymbol)}.
+      Variable mig : migrator Esymbol tus tus'.
+
+      Fixpoint wtgoal_subst {tvs tvs'}
+               (sVar : hlist (wtexpr Esymbol tus' tvs') tvs)
+               (gl : wtgoal tus tvs)
+      : wtgoal tus' tvs'.
+      refine
+        match gl with
+        | wtSolved => wtSolved
+        | wtGoal gl => wtGoal (subst sVar (migrate_expr mig gl))
+        | wtConj l r =>
+          wtConj (wtgoal_subst _ _ sVar l) (wtgoal_subst _ _ sVar r)
+        | wtHyp p g =>
+          wtHyp (subst sVar (migrate_expr mig p)) (wtgoal_subst _ _ sVar g)
+        | wtAll t g =>
+          wtAll t (wtgoal_subst _ _
+                                (Hcons (wtVar (Member.MZ _ _)) _) g)
+        end.
+      eapply hlist_map.
+      2: eapply sVar.
+      intros.
+      eapply (@wtexpr_lift _ _ tus' _ _ (_::nil) nil X).
+      Defined.
+    End wtgoal_subst.
+
+    Fixpoint wtgoalD {tus tvs} (g : wtgoal tus tvs) {struct g}
+    : exprT TsymbolD tus tvs (typeD TsymbolD tyProp) :=
+      match g with
+      | wtSolved => pure ltrue
+      | wtGoal g => wtexprD EsymbolD g
+      | wtConj l r =>
+        ap (ap (pure land) (wtgoalD l)) (wtgoalD r)
+      | wtHyp h g => ap (ap (pure limpl) (wtexprD EsymbolD h)) (wtgoalD g)
+      | @wtAll _ _ t g =>
+        let gD := wtgoalD g in
+        ap (T:=exprT TsymbolD tus tvs) (pure (@lforall _ _ (typeD TsymbolD t)))
+           (fun us vs v => gD us (Hcons v vs))
+      end.
+
+    Variables Pre Post : list (Tuvar Tsymbol) -> list (type Tsymbol) -> Type.
+
+    Record resultA tus resultUs tvs : Type := mkResultA
+    { result         : Post resultUs tvs
+    ; resultPrems    : list (wtexpr Esymbol resultUs tvs tyProp)
+    ; resultSubst    : Inst resultUs
+    ; resultMigrator : migrator Esymbol tus resultUs }.
+    Arguments mkResultA {_ _ _} _ _ _ _ : clear implicits.
+
+    Record resultC tus tvs : Type := mkResultC
+    { resultUs       : _
+    ; the_result     : resultA tus resultUs tvs }.
+    Arguments mkResultC {_ _ _} _ : clear implicits.
+
+    (** Statically known pre- and post-context
+     **)
+    Definition logicA tus tus' tvs : Type :=
+      forall
+        (prems : list (wtexpr Esymbol tus tvs tyProp))
+        (inst  : Inst tus)
+        (goal  : Pre tus tvs),
+        m (resultA tus tus' tvs).
+
+    (** Statically known pre- context
+     **)
+    Definition logicC tus tvs : Type :=
+      forall
+        (prems : list (wtexpr Esymbol tus tvs tyProp))
+        (inst  : Inst tus)
+        (goal  : Pre tus tvs),
+        m (resultC tus tvs).
+
+    (** NOTE: [logicT] does not form a monad due to the generalization
+     **       over the indices.
+     **)
+    Definition logicM : Type :=
+      forall tus tvs, logicC tus tvs.
+
+    Variable PreD
+    : forall {tus tvs}, Pre tus tvs ->
+                        exprT TsymbolD tus tvs (typeD TsymbolD tyProp).
+    Variable PostD
+    : forall {tus tvs}, Post tus tvs ->
+                        exprT TsymbolD tus tvs (typeD TsymbolD tyProp).
+
+    Context {Functor_m : Functor m}.
+    Context {FLogic_m : FLogic m}.
+
+    Definition logicA_spec {tus tus' tvs} (c : logicA tus tus' tvs) : Prop :=
+      forall prems goal inst result,
+        c prems inst goal = result ->
+        fmodels (fun t =>
+              match t with
+              | mkResultA post prems' inst' trans =>
+                Inst_evolves trans inst inst' /\
+                @foralls_uvar_prop tus' (fun us' =>
+                  let us := migrate_env EsymbolD trans us' in
+                  InstD inst' us' ->
+                  lentails ltrue
+                    (@foralls_prop tvs (fun vs =>
+                       limpl (impls_prop
+                                (map (fun p => wtexprD EsymbolD p us' vs) prems')
+                                (@PostD _ _ post us' vs))
+                             (impls_prop
+                                (map (fun p => wtexprD EsymbolD p us vs) prems)
+                                (@PreD  _ _ goal us  vs)))))
+              end)
+           result.
+
+    Definition logicC_spec {tus tvs} (c : logicC tus tvs) : Prop :=
+      forall prems goal inst result,
+        c prems inst goal = result ->
+        fmodels (fun t =>
+              match t with
+              | @mkResultC _ _ tus' (mkResultA post prems' inst' trans) =>
+                Inst_evolves trans inst inst' /\
+                @foralls_uvar_prop tus' (fun us' =>
+                  let us := migrate_env EsymbolD trans us' in
+                  InstD inst' us' ->
+                  lentails ltrue
+                    (@foralls_prop tvs (fun vs =>
+                       limpl (impls_prop
+                                (map (fun p => wtexprD EsymbolD p us' vs) prems')
+                                (@PostD _ _ post us' vs))
+                             (impls_prop
+                                (map (fun p => wtexprD EsymbolD p us vs) prems)
+                                (@PreD  _ _ goal us  vs)))))
+              end)
+           result.
+
+    Definition logicM_spec (l : logicM) : Prop :=
+      forall tus tvs,
+        logicC_spec (l tus tvs).
+  End logicM.
+
 
   Lemma foralls_uvar_prop_impl
     : forall ts (P Q : _ -> Prop),
@@ -218,11 +294,6 @@ Section simple_dep_types.
     eapply landL1. reflexivity.
   Qed.
 
-
-  Require Import MirrorCore.LambdaWt.Unify.
-  Require Import ExtLib.Structures.Monads.
-  Require Import ExtLib.Structures.Functor.
-
   Lemma wtexpr_equiv_Unifiable_eq
   : forall tus tvs t (e1 e2 : wtexpr Esymbol tus tvs t)
            (i : Inst tus),
@@ -255,6 +326,75 @@ Section simple_dep_types.
     { etransitivity;
       [ eapply IHwtexpr_equiv1 | eapply IHwtexpr_equiv2 ]; eauto. }
   Admitted.
+
+  Section evar_tactic.
+    Variable m : Type -> Type.
+    Context {Monad_m : Monad m}.
+    Context {Functor_m : Functor m}.
+
+    Variable unify : Unifier Esymbol Inst.
+    Variable unifyOk : UnifierOk unify.
+
+    Context {FLogic_m : FLogic m}.
+    Context {MLogic_m : MLogic m}.
+
+
+    Definition migrator_fresh t tus
+    : migrator Esymbol tus (tus ++ t :: nil).
+      eapply WtMigrator.migrator_id'. simpl.
+      intros. eapply wtUVar.
+      eapply DepUtil.member_lift with (ls'':=tus) (ls:=nil) (ls':=t::nil).
+      rewrite (app_nil_r_trans tus). eassumption.
+      eapply WtMigrator.vars_id.
+    Defined.
+
+    Definition Inst_fresh t {tus} (i : Inst tus)
+    : Inst (tus ++ t :: nil).
+    Admitted.
+
+    Variables Pre Post : list (Tuvar Tsymbol) -> list (type Tsymbol) -> Type.
+    Variable Pre_Post_migrate
+      : forall tus t tvs, Pre tus tvs -> Post (tus ++ t :: nil) tvs.
+
+    Definition Evar {tus tvs} t
+    : logicA m Pre Post tus (tus ++ t :: nil) tvs :=
+      fun prems sub goal =>
+        let mig := migrator_fresh t tus in
+        ret {| result := Pre_Post_migrate t goal
+             ; resultPrems := map (migrate_expr mig) prems
+             ; resultSubst := Inst_fresh t sub
+             ; resultMigrator := mig |}.
+  End evar_tactic.
+
+  Section under_tactic.
+    Variable m : Type -> Type.
+    Context {Monad_m : Monad m}.
+    Context {Functor_m : Functor m}.
+    Context {MonadZero_m : MonadZero m}.
+
+    Context {FLogic_m : FLogic m}.
+    Context {MLogic_m : MLogic m}.
+    Context {MLogicZero_m : MLogicZero m}.
+
+    Context {Post : list (Tuvar Tsymbol) -> list (type Tsymbol) -> Type}.
+    Definition Under_All {tus tvs}
+               (tac : forall t, logicC m wtgoal Post tus (t :: tvs))
+    : logicC m wtgoal Post tus tvs.
+    refine (
+        fun prems sub goal =>
+          match goal with
+          | @wtAll _ _ t goal' =>
+            (** TODO(gmalecha): This is going to be too expensive.
+             ** 1/ Combine prems and quantifiers into a context.
+             ** 2/ Might not want to eagerly instantiate premises
+             **)
+            fmap _ (tac t _ sub goal')
+          | _ => mzero
+          end).
+    admit. admit.
+    Admitted.
+  End under_tactic.
+
 
   Section assumption_tactic.
     Variable m : Type -> Type.
@@ -345,7 +485,7 @@ Section simple_dep_types.
 
     End find_premise.
 
-    Require Import ChargeCore.Tactics.Tactics.
+
     Lemma impls_prop_ap
       : forall P Q prems G,
         G |-- impls_prop prems (P -->> Q) ->
@@ -364,18 +504,18 @@ Section simple_dep_types.
 
 
     Definition Assumption
-    : logicT m
+    : logicM m
              (fun tus tvs => wtexpr Esymbol tus tvs tyProp)
              (fun _ _ => unit) :=
       fun tus tvs prems sub goal =>
         fmap (F:=m)
-             (fun sub' => mkResultC (fun _ _ => unit) tt prems sub' migrator_id)
+             (fun sub' => mkResultC (mkResultA (fun _ _ => unit) tt prems sub' migrator_id))
              (find_premise goal sub prems).
 
     Theorem Assumption_sound
-    : logicT_spec (fun tus tvs e => wtexprD EsymbolD e)
+    : logicM_spec (fun tus tvs e => wtexprD EsymbolD e)
                   (fun _ _ _ => Pure_exprT ltrue)
-                  fmodels Assumption.
+                  Assumption.
     Proof.
       red. red. unfold Assumption. intros.
       subst.
@@ -395,17 +535,64 @@ Section simple_dep_types.
     Qed.
   End assumption_tactic.
 
-  Section cut_tactic.
+  Section apply_tactic.
     Variable m : Type -> Type.
     Context {Monad_m : Monad m}.
-    Context {MonadPlus_m : MonadPlus m}.
     Context {MonadZero_m : MonadZero m}.
     Context {Functor_m : Functor m}.
 
     Context {FLogic_m : FLogic m}.
     Context {MLogic_m : MLogic m}.
-    Context {MLogicPlus_m : MLogicPlus m}.
     Context {MLogicZero_m : MLogicZero m}.
+
+    Variable unify : Unifier Esymbol Inst.
+    Variable unifyOk : UnifierOk unify.
+
+    Section lemma.
+      Variable C : list (Tuvar Tsymbol) -> list (type Tsymbol) -> Type.
+      Variable CD : forall {tus tvs},
+          C tus tvs -> exprT TsymbolD tus tvs (typeD TsymbolD tyProp).
+
+      Record lemma tus tvs : Type :=
+      { vars  : list (type Tsymbol)
+      ; prems : list (wtexpr Esymbol tus (vars ++ tvs) tyProp)
+      ; concl : C tus (vars ++ tvs)
+      }.
+
+      Definition lemmaD {tus tvs} (l : lemma tus tvs)
+      : exprT TsymbolD tus tvs (typeD TsymbolD tyProp) :=
+        fun us vs =>
+          foralls_prop
+            (fun vs' : Venv TsymbolD l.(vars) =>
+               impls_prop
+                 (map (fun e => wtexprD EsymbolD e us (hlist_app vs' vs))
+                      l.(prems))
+                 (CD l.(concl) us (hlist_app vs' vs))).
+    End lemma.
+(*
+    Definition EApply {tus tvs}
+               (lem : lemma (fun tus tvs => wtexpr Esymbol tus tvs tyProp) tus tvs)
+    : logicC m
+             (fun tus tvs => wtexpr Esymbol tus tvs tyProp)
+             (fun tus tvs => wtgoal tus tvs)%type
+             tus tvs.
+    refine (
+      fun prems sub goal =>
+        match unify goal lem.(concl) sub with
+        | None => mzero
+        | Some sub' => _
+        end).
+*)
+
+  End apply_tactic.
+
+  Section cut_tactic.
+    Variable m : Type -> Type.
+    Context {Monad_m : Monad m}.
+    Context {Functor_m : Functor m}.
+
+    Context {FLogic_m : FLogic m}.
+    Context {MLogic_m : MLogic m}.
 
     Definition Cut {tus tvs} (t : wtexpr Esymbol tus tvs tyProp)
     : logicC m
@@ -413,11 +600,12 @@ Section simple_dep_types.
              (fun tus tvs => wtgoal tus tvs)%type
              tus tvs :=
       fun prems sub goal =>
-        ret (m:=m) (mkResultC wtgoal
-                              (wtConj (wtGoal t) (wtHyp t (wtGoal goal)))
-                              prems
-                              sub
-                              migrator_id).
+        ret (m:=m) (mkResultC
+                      (mkResultA wtgoal
+                                 (wtConj (wtGoal t) (wtHyp t (wtGoal goal)))
+                                 prems
+                                 sub
+                                 migrator_id)).
 
     Existing Instance Reflexive_Inst_evolves.
 
@@ -425,7 +613,6 @@ Section simple_dep_types.
     : forall tus tvs t,
         logicC_spec (fun tus tvs e => wtexprD EsymbolD e)
                     (fun _ _ e => @wtgoalD _ _ e)
-                    fmodels
                     (@Cut tus tvs t).
     Proof.
       unfold Cut. red. simpl; intros. subst.
@@ -449,7 +636,7 @@ End simple_dep_types.
 
 
 (*
-    Definition logicT_cps (Pre Post : _ -> _ -> Type) : Type :=
+    Definition logicM_cps (Pre Post : _ -> _ -> Type) : Type :=
       forall tus tvs
         (prems : list (wtexpr Esymbol tus tvs tyProp))
         (goal  : Pre tus tvs)
